WIP. fix IndexedInvSet

src/tlogic/IndexedInvariants.v
@@ -130,6 +130,313 @@ Section WORLD_SATISFACTION.
                      n (@Auth.black (positive ==> URA.agree Var)%ra
                                     (fun (i : positive) => Some <$> (I !! i))).
 
+  Definition inv_auth (I : gmap positive Var) := OwnM (inv_auth_black I).
+
+  (* Definition inv_satall (I : gmap positive Var) := *)
+  (*   ([∗ map] i ↦ p ∈ I, (prop p) ∗ OwnD n {[i]} ∨ OwnE n {[i]})%I. *)
+  Definition inv_satall (I : gmap positive Var) :=
+    ([∗ map] i ↦ p ∈ I, (prop n p) ∗ OwnD n {[i]} ∨ OwnE n {[i]})%I.
+
+  Definition wsat : iProp := (∃ I, inv_auth I ∗ inv_satall I)%I.
+
+
+  Lemma alloc_name φ
+        (INF : forall (E : index -> option (gset positive)) n,
+            match E n with
+            | None => True
+            | Some G => (exists i, i ∉ G /\ φ i)
+            end)
+    : ⊢ |==> ∃ i, ⌜φ i⌝ ∧ OwnD n {[i]}.
+  Proof.
+    assert (@URA.updatable_set
+              (index ==> Gset.t)%ra
+              (fun _ => (Some ∅ : Gset.t))
+              (fun r => exists i, r = (maps_to_res n (Some {[i]} : Gset.t)) /\ φ i)) as UPD.
+    { clear - INF. ii. apply URA.wf_split in WF; des. specialize (INF ctx n).
+      des_ifs.
+      - des. esplits; eauto.
+        unfold maps_to_res, URA.wf, URA.add. unseal "ra". ss.
+        i. des_ifs.
+        + unfold URA.wf, URA.add in *. unseal "ra". ss.
+          specialize (WF0 n). unfold URA.wf in WF0. unseal "ra". ss. des_ifs. set_solver.
+        + rewrite URA.unit_idl. unfold URA.wf in WF0. unseal "ra". ss.
+      - rr in WF0. unseal "ra". ss. specialize (WF0 n). rr in WF0. unseal "ra". ss.
+        rewrite Heq in WF0. ss.
+    }
+    (* iPoseProof (@OwnM_unit _ _ H0) as "-# H". *)
+    iPoseProof (@OwnM_unit _ _ H1) as "-# H".
+    iMod (OwnM_Upd_set UPD with "H") as "[% [% DIS]]".
+    iModIntro. des. subst. iExists i. eauto.
+  Qed.
+
+  Lemma wsat_OwnI_alloc p φ
+        (INF : forall (E : index -> option (gset positive)) n,
+            match E n with
+            | None => True
+            | Some G => (exists i, i ∉ G /\ φ i)
+            end)
+    (* : wsat ∗ prop p ⊢ |==> (∃ i, ⌜φ i⌝ ∧ OwnI n i p) ∗ wsat. *)
+    : wsat ∗ prop n p ⊢ |==> (∃ i, ⌜φ i⌝ ∧ OwnI n i p) ∗ wsat.
+  Proof.
+    iIntros "[[% [AUTH SAT]] P]".
+    iMod (alloc_name (fun i => i ∉ dom I /\ φ i)) as "[% [[%iI %iφ] D]]".
+    { i.
+      set (uni := fun n => match E n with
+                        | None => None
+                        | Some G => Some (G ∪ dom I)
+                        end).
+      specialize (INF uni n0). subst uni. ss. des_ifs.
+      des. eapply not_elem_of_union in INF. des. esplits; eauto. }
+    pose (<[i:=p]> I) as I'.
+
+    assert (URA.updatable
+              (maps_to_res_dep n (@Auth.black (positive ==> URA.agree Var)%ra (fun i => Some <$> (I !! i))) : IInvSetRA Vars)
+              ((maps_to_res_dep n (@Auth.black (positive ==> URA.agree Var)%ra (fun i => Some <$> (I' !! i))) : IInvSetRA Vars)
+                 ⋅
+                 (maps_to_res_dep n (Auth.white (@maps_to_res _ (URA.agree Var) i (Some (Some p)))) : IInvSetRA Vars))).
+    { setoid_rewrite maps_to_res_dep_add. apply maps_to_res_dep_updatable.
+      apply Auth.auth_alloc. ii. des. rewrite URA.unit_idl in FRAME. subst. split.
+      { rr; unseal "ra". ss. intro. rr; unseal "ra". destruct (I' !! k); ss. }
+      rr. subst I'.
+      unfold URA.add. unseal "ra". ss.
+      extensionalities j. unfold maps_to_res. des_ifs.
+      - rewrite lookup_insert. rewrite not_elem_of_dom_1; ss.
+        unfold URA.add. unseal "ra". ss.
+      - rewrite URA.unit_idl. rewrite lookup_insert_ne; eauto.
+    }
+    unfold inv_auth, inv_satall.
+    (* iMod (OwnM_Upd H2 with "AUTH") as "[AUTH NEW]". iModIntro. *)
+    iMod (OwnM_Upd H3 with "AUTH") as "[AUTH NEW]". iModIntro.
+
+    iSplit.
+    - iExists i. iFrame. ss.
+    - unfold wsat. iExists I'. iFrame.
+      unfold inv_satall. subst I'.
+      iApply big_sepM_insert.
+      { apply not_elem_of_dom_1; ss. }
+      iSplitL "P D"; ss. iLeft. iFrame.
+  Qed.
+
+  Lemma wsat_OwnI_open i p :
+    (* OwnI n i p ∗ wsat ∗ OwnE n {[i]} ⊢ |==> prop p ∗ wsat ∗ OwnD n {[i]}. *)
+    OwnI n i p ∗ wsat ∗ OwnE n {[i]} ⊢ |==> prop n p ∗ wsat ∗ OwnD n {[i]}.
+  Proof.
+    iIntros "(I & [% [AUTH SAT]] & EN)". iModIntro.
+    unfold OwnI, inv_auth, inv_satall.
+    iCombine "AUTH I" as "AUTH".
+    iPoseProof (OwnM_valid with "AUTH") as "%WF".
+    assert (Hip : I !! i = Some p).
+    { unfold inv_auth_black, OwnI_white in WF. setoid_rewrite maps_to_res_dep_add in WF.
+      unfold maps_to_res_dep, maps_to_res in WF. apply (pwd_lookup_wf n) in WF. ss. des_ifs.
+      unfold eq_rect_r in WF. rewrite <- Eqdep.EqdepTheory.eq_rect_eq in WF.
+      apply Auth.auth_included in WF. rename WF into EXTENDS.
+      apply pw_extends in EXTENDS. specialize (EXTENDS i).
+      des_ifs. clear e e0. rr in EXTENDS. des. unfold URA.add in EXTENDS; unseal "ra".
+      destruct (I !! i) eqn: E.
+      - destruct ctx; ss; des_ifs.
+      - destruct ctx; ss; des_ifs.
+    }
+    clear WF.
+    iDestruct "AUTH" as "[AUTH I]".
+    iPoseProof (big_sepM_delete _ _ _ _ Hip with "SAT") as "[[[H1 H2]|H1] SAT]".
+    2: { iCombine "EN H1" as "F". iPoseProof (OwnM_valid with "F") as "%WF".
+         exfalso. unfold maps_to_res, URA.wf, URA.add in WF. unseal "ra". ss.
+         specialize (WF n). des_ifs. unfold URA.wf, URA.add in WF. unseal "ra".
+         ss. des_ifs. set_solver.
+    }
+    iFrame. unfold wsat. iExists I. iFrame. unfold inv_satall.
+    iApply (big_sepM_delete _ _ _ _ Hip). iFrame.
+  Qed.
+
+  Lemma wsat_OwnI_close i p :
+    (* OwnI n i p ∗ wsat ∗ prop p ∗ OwnD n {[i]} ⊢ |==> wsat ∗ OwnE n {[i]}. *)
+    OwnI n i p ∗ wsat ∗ prop n p ∗ OwnD n {[i]} ⊢ |==> wsat ∗ OwnE n {[i]}.
+  Proof.
+    iIntros "(I & [% [AUTH SAT]] & P & DIS)". iModIntro.
+    unfold OwnI, inv_auth, inv_satall.
+    iCombine "AUTH I" as "AUTH".
+    iPoseProof (OwnM_valid with "AUTH") as "%WF".
+    assert (Hip : I !! i = Some p).
+    { unfold inv_auth_black, OwnI_white in WF. setoid_rewrite maps_to_res_dep_add in WF.
+      unfold maps_to_res_dep, maps_to_res in WF. apply (pwd_lookup_wf n) in WF. ss. des_ifs.
+      unfold eq_rect_r in WF. rewrite <- Eqdep.EqdepTheory.eq_rect_eq in WF.
+      apply Auth.auth_included in WF. rename WF into EXTENDS.
+      apply pw_extends in EXTENDS. specialize (EXTENDS i).
+      des_ifs. clear e e0.
+      rr in EXTENDS. des. unfold URA.add in EXTENDS; unseal "ra".
+      destruct (I !! i) eqn: E.
+      - destruct ctx; ss; des_ifs.
+      - destruct ctx; ss; des_ifs.
+    }
+    clear WF.
+    iDestruct "AUTH" as "[AUTH I]".
+    iPoseProof (big_sepM_delete _ _ _ _ Hip with "SAT") as "[[[H1 H2]|H1] SAT]".
+    { iCombine "DIS H2" as "F". iPoseProof (OwnM_valid with "F") as "%WF".
+      exfalso. unfold maps_to_res, URA.wf, URA.add in WF. unseal "ra". ss.
+      specialize (WF n). des_ifs.
+      unfold URA.wf, URA.add in WF. unseal "ra". ss. des_ifs. set_solver.
+    }
+    iFrame. unfold wsat. iExists I. iFrame. unfold inv_satall.
+    iApply (big_sepM_delete _ _ _ _ Hip). iFrame. iLeft. iFrame.
+  Qed.
+
+  Lemma wsat_init :
+    OwnM (maps_to_res_dep n (@Auth.black (positive ==> URA.agree Var)%ra (fun (i : positive) => None)))
+      ⊢ wsat.
+  Proof.
+    iIntros "H". iExists ∅. iFrame.
+    unfold inv_satall. iApply big_sepM_empty. ss.
+  Qed.
+
+End WORLD_SATISFACTION.
+
+Section WSATS.
+
+  Context `{Σ : GRA.t}.
+  Context `{Vars : index -> Type}.
+  Context `{@IInvSet Σ Vars}.
+  Context `{@GRA.inG (index ==> CoPset.t)%ra Σ}.
+  Context `{@GRA.inG (index ==> Gset.t)%ra Σ}.
+  Context `{@GRA.inG (IInvSetRA Vars) Σ}.
+
+  Definition wsat_auth_black (N : gset index) : IInvSetRA Vars :=
+    (fun n => if (gset_elem_of_dec n N)
+           then ε
+           else @Auth.black (positive ==> URA.agree (Vars n))%ra (fun _ => None)).
+
+  Definition wsat_auth (N : gset index) := OwnM (wsat_auth_black N).
+
+  Definition wsat_satall (N : gset index) := ([∗ set] n ∈ N, wsat n)%I.
+
+  Definition wsats : iProp := (∃ N, wsat_auth N ∗ wsat_satall N)%I.
+
+  Lemma wsat_auth_nin (N : gset index) (n : index) (NIN : n ∉ N)
+    : wsat_auth N ⊢ |==> wsat_auth ({[n]} ∪ N) ∗ wsat n.
+  Proof.
+    iIntros "AUTH".
+    remember ({[n]} ∪ N) as N'.
+    assert (URA.updatable
+              (wsat_auth_black N)
+              ((wsat_auth_black N')
+                 ⋅
+                 (maps_to_res_dep n (@Auth.black (positive ==> URA.agree (Vars n))%ra (fun (i : positive) => None))))).
+    { apply pointwise_dep_updatable. i.
+      unfold wsat_auth_black, maps_to_res_dep. unfold URA.add. unseal "ra". ss.
+      destruct (excluded_middle_informative (a = n)).
+      - subst a. des_ifs.
+        2:{ exfalso. set_solver + n1. }
+        unfold eq_rect_r. ss. rewrite URA.unit_idl. reflexivity.
+      - subst N'. destruct (gset_elem_of_dec a N).
+        { des_ifs.
+          - rewrite URA.unit_idl. reflexivity.
+          - exfalso. set_solver + e n1.
+        }
+        { des_ifs.
+          - set_solver + n0 n1 e.
+          - rewrite URA.unit_id. reflexivity.
+        }
+    }
+    unfold wsat_auth.
+    iMod (OwnM_Upd H3 with "AUTH") as "[AUTH NEW]".
+    iPoseProof (wsat_init with "NEW") as "NEW".
+    iModIntro. iFrame.
+  Qed.
+
+  Lemma wsat_satall_nin (N : gset index) (n : index) (NIN : n ∉ N)
+    : wsat_satall N ∗ wsat n ⊢ wsat_satall ({[n]} ∪ N).
+  Proof.
+    iIntros "[SALL WSAT]". unfold wsat_satall. iApply (big_sepS_insert); auto. iFrame.
+  Qed.
+
+
+  Lemma wsats_OwnI_alloc n p φ
+        (INF : forall (E : index -> option (gset positive)) n,
+            match E n with
+            | None => True
+            | Some G => (exists i, i ∉ G /\ φ i)
+            end)
+    : wsats ∗ prop n p ⊢ |==> (∃ i, ⌜φ i⌝ ∧ OwnI n i p) ∗ wsats.
+  Proof.
+    iIntros "[[% [AUTH SALL]] P]".
+    destruct (gset_elem_of_dec n N).
+    { iPoseProof (big_sepS_elem_of_acc with "SALL") as "[WSAT K]". apply e.
+      iPoseProof (wsat_OwnI_alloc with "[WSAT P]") as ">[RES WSAT]". apply INF. iFrame.
+      iPoseProof ("K" with "WSAT") as "SALL".
+      iModIntro. iFrame. iExists _. iFrame.
+    }
+    { iMod (wsat_auth_nin with "AUTH") as "[AUTH WSAT]". apply n0.
+      iPoseProof (wsat_OwnI_alloc with "[WSAT P]") as ">[RES WSAT]". apply INF. iFrame.
+      iPoseProof (wsat_satall_nin with "[SALL WSAT]") as "SALL". apply n0. iFrame.
+      iModIntro. iFrame. iExists _. iFrame.
+    }
+  Qed.
+
+  Lemma wsats_OwnI_open n i p :
+    OwnI n i p ∗ wsats ∗ OwnE n {[i]} ⊢ |==> prop n p ∗ wsats ∗ OwnD n {[i]}.
+  Proof.
+    iIntros "(I & [% [AUTH SAT]] & EN)".
+    unfold OwnI, wsat_auth, wsat_satall.
+    iCombine "AUTH I" as "AUTH".
+    iPoseProof (OwnM_valid with "AUTH") as "%WF".
+    assert (Hin : n ∈ N).
+    { unfold wsat_auth_black, OwnI_white, maps_to_res_dep in WF. unfold URA.add in WF. unseal "ra". ss.
+      apply (pwd_lookup_wf n) in WF. ss. des_ifs.
+      exfalso. unfold eq_rect_r in WF. rewrite <- Eqdep.EqdepTheory.eq_rect_eq in WF.
+      unfold maps_to_res in WF. apply Auth.auth_included in WF. rename WF into EXTENDS.
+      apply pw_extends in EXTENDS. specialize (EXTENDS i). des_ifs.
+      clear e e0. rr in EXTENDS. des. unfold URA.add in EXTENDS; unseal "ra".
+      ss. des_ifs.
+    }
+    clear WF. iDestruct "AUTH" as "[AUTH I]".
+    iPoseProof (big_sepS_elem_of_acc with "SAT") as "[WSAT K]". apply Hin.
+    iMod (wsat_OwnI_open with "[I WSAT EN]") as "[P [WSAT DN]]". iFrame.
+    iPoseProof ("K" with "WSAT") as "SAT".
+    iModIntro. iFrame. iExists _. iFrame.
+  Qed.
+
+  Lemma wsats_OwnI_close n i p :
+    OwnI n i p ∗ wsats ∗ prop n p ∗ OwnD n {[i]} ⊢ |==> wsats ∗ OwnE n {[i]}.
+  Proof.
+
+
+    TODO
+
+    iIntros "(I & [% [AUTH SAT]] & P & DIS)". iModIntro.
+    unfold OwnI, inv_auth, inv_satall.
+    iCombine "AUTH I" as "AUTH".
+    iPoseProof (OwnM_valid with "AUTH") as "%WF".
+    assert (Hip : I !! i = Some p).
+    { unfold inv_auth_black, OwnI_white in WF. setoid_rewrite maps_to_res_dep_add in WF.
+      unfold maps_to_res_dep, maps_to_res in WF. apply (pwd_lookup_wf n) in WF. ss. des_ifs.
+      unfold eq_rect_r in WF. rewrite <- Eqdep.EqdepTheory.eq_rect_eq in WF.
+      apply Auth.auth_included in WF. rename WF into EXTENDS.
+      apply pw_extends in EXTENDS. specialize (EXTENDS i).
+      des_ifs. clear e e0.
+      rr in EXTENDS. des. unfold URA.add in EXTENDS; unseal "ra".
+      destruct (I !! i) eqn: E.
+      - destruct ctx; ss; des_ifs.
+      - destruct ctx; ss; des_ifs.
+    }
+    clear WF.
+    iDestruct "AUTH" as "[AUTH I]".
+    iPoseProof (big_sepM_delete _ _ _ _ Hip with "SAT") as "[[[H1 H2]|H1] SAT]".
+    { iCombine "DIS H2" as "F". iPoseProof (OwnM_valid with "F") as "%WF".
+      exfalso. unfold maps_to_res, URA.wf, URA.add in WF. unseal "ra". ss.
+      specialize (WF n). des_ifs.
+      unfold URA.wf, URA.add in WF. unseal "ra". ss. des_ifs. set_solver.
+    }
+    iFrame. unfold wsat. iExists I. iFrame. unfold inv_satall.
+    iApply (big_sepM_delete _ _ _ _ Hip). iFrame. iLeft. iFrame.
+  Qed.
+
+
+  REF
+
+  Definition inv_auth_black (I : gmap positive Var) : IInvSetRA Vars :=
+    @maps_to_res_dep index _
+                     n (@Auth.black (positive ==> URA.agree Var)%ra
+                                    (fun (i : positive) => Some <$> (I !! i))).
+
   Definition inv_auth (I : gmap positive Var) :=
     OwnM (inv_auth_black I).
 
@@ -289,7 +596,7 @@ Section WORLD_SATISFACTION.
     unfold inv_satall. iApply big_sepM_empty. ss.
   Qed.
 
-End WORLD_SATISFACTION.
+End WSATS.
 
 Section FANCY_UPDATE.
 
